Coq/src/SimRelAddEW.v
@@ -30,7 +30,7 @@ Set Implicit Arguments.
 Local Open Scope program_scope.
 
 Section SimRelAddEW.
-  Variable prog : Prog.t.
+  Variable prog : stable_prog_type.
   Variable G : execution.
   Variable sc : relation actid.
   Variable TC : trav_config.
