Coq/src/SimRelCertStepCoh.v
@@ -38,7 +38,7 @@ Local Open Scope program_scope.
 
 Section SimRelCertStepCoh.
 
-  Variable prog : Prog.t.
+  Variable prog : stable_prog_type.
   Variable G : execution.
   Variable sc : relation actid.
   Variable TC : trav_config.
@@ -361,7 +361,7 @@ Section SimRelCertStepCoh.
     assert (ES.Wf S) as WF by apply SRCC.
     assert (ES.Wf S') as WFS.
     { eapply simrel_cert_step_wf; eauto. }
-    assert (simrel_cont prog S' G TC) as SRCONT.
+    assert (simrel_cont (stable_prog_to_prog prog) S' G TC) as SRCONT.
     { eapply basic_step_simrel_cont; try apply SRCC; eauto. 
       eapply cstate_covered; eauto. }
     assert (simrel_e2a S' G sc) as SRE2A.
@@ -430,7 +430,8 @@ Section SimRelCertStepCoh.
 
     assert (e2a S' □ Ssb S' ⊆ Gsb) as SBN.
     { eapply e2a_sb; eauto; try apply SRCC.
-      eapply e2a_GE; eauto. }
+      2: by eapply e2a_GE; eauto.
+      apply stable_prog_to_prog_no_init; apply SRCC. }
     
     assert (e2a S' □ Shb S' ⊆ Ghb) as HBN.
     { eapply e2a_hb; eauto; apply SRCC. }
